SMT representation for memory programs.

CrVal.v
@@ -1,88 +1,221 @@
+Require Import ZArith.
 From MyProject Require Import MyInts.
 From MyProject Require Import Integers.
+From MyProject Require Import Maps.
 
+Inductive Check_T (T : Type) :=
+| Legal (v : T)
+| Illegal.
+Arguments Legal {T} _.
+Arguments Illegal {T}.
+
+Inductive CrInt_T : Type :=
+| CrUInt8 (val : uint8)
+| CrUInt32 (val : uint32)
+| CrNilInt.
+Inductive CrPtr_T : Type :=
+| CrPtr (base : uintptr) (idx : uintptr)
+| CrNilPtr.
 Inductive CrVal : Type :=
-| CrInt (val : uint8)
-| CrPtr (base : uintptr) (offset : uintptr)
-| CrNil.
+| IntVal (val : CrInt_T)
+| PtrVal (val : CrPtr_T)
+| UninitVal
+| ErrorVal.
+
+Inductive MemVal (T : Type) :=
+| Init (v : T)
+| Uninit.
+Arguments Init {T} _.
+Arguments Uninit {T}.
+Record MemBlock (T : Type) := {
+  arr_len : uint32;
+  arr_bytes : PMap.t (MemVal T);
+}.
+Arguments arr_len {T} _.
+Arguments arr_bytes {T} _.
+Inductive Array {T : Type} :=
+| Allocated (arr : MemBlock T)
+| Unallocated.
+Arguments Unallocated {T}.
+Inductive Memory (T : Type) :=
+| Mem (m : PMap.t (@Array T))
+| Invalid.
+Arguments Mem {T} _.
+Arguments Invalid {T}.
+
+(* requires S to prevent collision @ 0 *)
+Definition pkey_to_mkey (p : uintptr) : positive :=
+  Pos.of_nat (S (Z.to_nat (unsigned p))).
 
 Definition eqb (x y : CrVal) : bool :=
   match x, y with
-  | CrInt x', CrInt y' => Integers.eq x' y'
-  | CrPtr b1 o1, CrPtr b2 o2 =>
+  | IntVal (CrUInt8 x'), IntVal (CrUInt8 y')
+  | IntVal (CrUInt32 x'), IntVal (CrUInt32 y') => Integers.eq x' y'
+  | PtrVal (CrPtr b1 o1), PtrVal (CrPtr b2 o2) =>
     (Integers.eq b1 b2) &&
     (Integers.eq o1 o2)
-  | CrNil, CrNil => true
+  | UninitVal, UninitVal
+  | ErrorVal, ErrorVal
+  | IntVal (CrNilInt), IntVal (CrNilInt)
+  | PtrVal (CrNilPtr), PtrVal (CrNilPtr) => true
   | _, _ => false
   end.
 
-Definition add (x y : CrVal) : CrVal :=
+Definition add (x y : CrVal) : Check_T CrVal :=
   match x, y with
-  | CrInt x', CrInt y' =>
-    (CrInt (Integers.add x' y'))
-  | CrPtr b' o', CrInt y_ =>
-    let y' : uintptr := repr (intval y_) in
-    (CrPtr b' (Integers.add o' y'))
-  | _, _ => CrNil
+  | IntVal (CrUInt8 x'), IntVal (CrUInt8 y')
+    => Legal (IntVal (CrUInt8 (Integers.add x' y')))
+  | IntVal (CrUInt32 x'), IntVal (CrUInt32 y')
+    => Legal (IntVal (CrUInt32 (Integers.add x' y')))
+  | PtrVal (CrPtr b' o'), IntVal (CrUInt32 y_)
+    => let y' : uintptr := repr (intval y_) in
+       Legal (PtrVal (CrPtr b' (Integers.add o' y')))
+  | _, _ => Illegal
   end.
 
-Definition sub (x y : CrVal) : CrVal :=
+Definition sub (x y : CrVal) : Check_T CrVal :=
   match x, y with
-  | CrInt x', CrInt y' =>
-    (CrInt (Integers.sub x' y'))
-  | CrPtr b' o', CrInt y_ =>
-    let y' : uintptr := repr (intval y_) in
-    (CrPtr b' (Integers.sub o' y'))
-  | _, _ => CrNil
+  | IntVal (CrUInt8 x'), IntVal (CrUInt8 y')
+    => Legal (IntVal (CrUInt8 (Integers.sub x' y')))
+  | IntVal (CrUInt32 x'), IntVal (CrUInt32 y')
+    => Legal (IntVal (CrUInt32 (Integers.sub x' y')))
+  (* | PtrVal (CrPtr b' o'), IntVal (CrUInt32 y_)
+    => let y' : uintptr := repr (intval y_) in
+       Legal (PtrVal (CrPtr b' (Integers.sub o' y'))) *)
+  | _, _ => Illegal
   end.
 
-Definition and (x y : CrVal) : CrVal :=
+Definition and (x y : CrVal) : Check_T CrVal :=
   match x, y with
-  | CrInt x', CrInt y' =>
-    (CrInt (Integers.and x' y'))
-  | _, _ => CrNil
+  | IntVal (CrUInt8 x'), IntVal (CrUInt8 y')
+    => Legal (IntVal (CrUInt8 (Integers.and x' y')))
+  | IntVal (CrUInt32 x'), IntVal (CrUInt32 y')
+    => Legal (IntVal (CrUInt32 (Integers.and x' y')))
+  | _, _ => Illegal
   end.
 
-Definition or (x y : CrVal) : CrVal :=
+Definition or (x y : CrVal) : Check_T CrVal :=
   match x, y with
-  | CrInt x', CrInt y' =>
-    (CrInt (Integers.or x' y'))
-  | _, _ => CrNil
+  | IntVal (CrUInt8 x'), IntVal (CrUInt8 y')
+    => Legal (IntVal (CrUInt8 (Integers.or x' y')))
+  | IntVal (CrUInt32 x'), IntVal (CrUInt32 y')
+    => Legal (IntVal (CrUInt32 (Integers.or x' y')))
+  | _, _ => Illegal
   end.
 
-Definition xor (x y : CrVal) : CrVal :=
+Definition xor (x y : CrVal) : Check_T CrVal :=
   match x, y with
-  | CrInt x', CrInt y' =>
-    (CrInt (Integers.xor x' y'))
-  | _, _ => CrNil
+  | IntVal (CrUInt8 x'), IntVal (CrUInt8 y')
+    => Legal (IntVal (CrUInt8 (Integers.xor x' y')))
+  | IntVal (CrUInt32 x'), IntVal (CrUInt32 y')
+    => Legal (IntVal (CrUInt32 (Integers.xor x' y')))
+  | _, _ => Illegal
   end.
 
-Definition not (x : CrVal) : CrVal :=
+Definition not (x : CrVal) : Check_T CrVal :=
   match x with
-  | CrInt x' =>
-    (CrInt (Integers.not x'))
-  | _ => CrNil
+  | IntVal (CrUInt8 x')
+    => Legal (IntVal (CrUInt8 (Integers.not x')))
+  | IntVal (CrUInt32 x')
+    => Legal (IntVal (CrUInt32 (Integers.not x')))
+  | _ => Illegal
   end.
 
-Definition mul (x y : CrVal) : CrVal :=
+Definition mul (x y : CrVal) : Check_T CrVal :=
   match x, y with
-  | CrInt x', CrInt y' =>
-    (CrInt (Integers.mul x' y'))
-  | _, _ => CrNil
+  | IntVal (CrUInt8 x'), IntVal (CrUInt8 y')
+    => Legal (IntVal (CrUInt8 (Integers.mul x' y')))
+  | IntVal (CrUInt32 x'), IntVal (CrUInt32 y')
+    => Legal (IntVal (CrUInt32 (Integers.mul x' y')))
+  | _, _ => Illegal
   end.
 
-Definition divu (x y : CrVal) : CrVal :=
+Definition divu (x y : CrVal) : Check_T CrVal :=
   match x, y with
-  | CrInt x', CrInt y' =>
-    (CrInt (Integers.divu x' y'))
-  | _, _ => CrNil
+  | IntVal (CrUInt8 x'), IntVal (CrUInt8 y')
+    => Legal (IntVal (CrUInt8 (Integers.divu x' y')))
+  | IntVal (CrUInt32 x'), IntVal (CrUInt32 y')
+    => Legal (IntVal (CrUInt32 (Integers.divu x' y')))
+  | _, _ => Illegal
   end.
 
-Definition modu (x y : CrVal) : CrVal :=
+Definition modu (x y : CrVal) : Check_T CrVal :=
   match x, y with
-  | CrInt x', CrInt y' =>
-    (CrInt (Integers.modu x' y'))
-  | _, _ => CrNil
+  | IntVal (CrUInt8 x'), IntVal (CrUInt8 y')
+    => Legal (IntVal (CrUInt8 (Integers.modu x' y')))
+  | IntVal (CrUInt32 x'), IntVal (CrUInt32 y')
+    => Legal (IntVal (CrUInt32 (Integers.modu x' y')))
+  | _, _ => Illegal
+  end.
+
+Definition ld (m : Memory CrVal) (p : CrVal) : Check_T CrVal :=
+  match m with
+  | Mem m' => 
+    match p with
+    | PtrVal (CrPtr base idx) =>
+      match m' !! (pkey_to_mkey base) with
+      | Allocated array => if (Integers.ltu idx (arr_len array)) then
+          match (arr_bytes array) !! (pkey_to_mkey idx) with
+          | Init v => Legal v
+          | Uninit => Legal UninitVal
+          end
+        else
+          Illegal
+      | Unallocated => Illegal
+      end
+    | _ => Illegal
+    end
+  | Invalid => Illegal
+  end.
+
+Definition st (m : Memory CrVal) (p : CrVal) (v : CrVal) : Check_T (Memory CrVal) :=
+  match m with
+  | Mem m' =>
+    match p with
+    | PtrVal (CrPtr base idx) =>
+      match m' !! (pkey_to_mkey base) with
+      | Allocated array => if (Integers.ltu idx (arr_len array)) then
+          Legal (Mem (PMap.set (pkey_to_mkey base) (Allocated {|
+            arr_len := arr_len array;
+            arr_bytes := PMap.set (pkey_to_mkey idx) (Init v) (arr_bytes array);
+          |}) m'))
+        else
+          Illegal
+      | Unallocated => Illegal
+      end
+    | _ => Illegal
+    end
+  | Invalid => Illegal
+  end.
+
+Definition tabula_rasa {T : Type} : Memory T :=
+  Mem (PMap.init Unallocated).
+
+(* TODO: Handle allocation collisions i.e. set mem to Invalid *)
+Definition alloc {T : Type} (m : Memory T) (arg1 : CrVal) : Check_T (Memory T) :=
+  match m with
+  | Mem m' =>
+    match arg1 with
+    | PtrVal (CrPtr b l) => Legal (Mem
+        (PMap.set (pkey_to_mkey b) (Allocated {|
+          arr_len := l;
+          arr_bytes := PMap.init Uninit;
+      |}) m'))
+    | _ => Illegal
+    end
+  | Invalid => Illegal
+  end.
+
+(* TODO: Handle double free *)
+Definition free {T : Type} (m : Memory T) (arg1 : CrVal) : Check_T (Memory T) :=
+  match m with
+  | Mem m' =>
+    match arg1 with
+    | PtrVal (CrPtr b _) => Legal (Mem
+        (PMap.set (pkey_to_mkey b) Unallocated m'))
+    | _ => Illegal
+    end
+  | Invalid => Illegal
   end.
 
 Lemma crval_concrete_if_else : forall (v1 v2 : CrVal),
@@ -90,42 +223,43 @@ Lemma crval_concrete_if_else : forall (v1 v2 : CrVal),
   v1 = v2.
 Proof.
   intros v1 v2 H.
-  destruct v1, v2; try discriminate.
-  - unfold eqb in H.
-    unfold eq in H.
-    unfold Rocqlib.zeq in H.
-    destruct (BinInt.Z.eq_dec (unsigned val) (unsigned val0)).
-    + apply uintw_eq_from_unsigned in e.
-      rewrite e.
-      reflexivity.
-    + exfalso. congruence.
-  - unfold eqb in H.
-    unfold eq in H.
-    unfold Rocqlib.zeq in H.
-    destruct (BinInt.Z.eq_dec (unsigned base) (unsigned base0));
-    destruct (BinInt.Z.eq_dec (unsigned offset) (unsigned offset0));
-    simpl in *.
-    + apply uintw_eq_from_unsigned in e.
-      apply uintw_eq_from_unsigned in e0.
-      rewrite e. rewrite e0. reflexivity.
-    + exfalso. congruence.
-    + exfalso. congruence.
-    + exfalso. congruence.
-  - reflexivity.
+  unfold eqb, eq, Rocqlib.zeq in H.
+  destruct v1, v2; try reflexivity; try discriminate;
+  try (destruct val; exfalso; congruence).
+  - destruct val; destruct val0; try discriminate; try reflexivity;
+    destruct (BinInt.Z.eq_dec (unsigned val) (unsigned val0)); try discriminate;
+    apply uintw_eq_from_unsigned in e; rewrite e; reflexivity.
+  - destruct val, val0; try discriminate; try reflexivity.
+    destruct (BinInt.Z.eq_dec (unsigned base) (unsigned base0)); try discriminate.
+    destruct (BinInt.Z.eq_dec (unsigned idx) (unsigned idx0)); try discriminate.
+    apply uintw_eq_from_unsigned in e, e0.
+    rewrite e, e0; reflexivity.
 Qed.
 
 Lemma crval_concrete_if_else2 : forall (v1 v2 : CrVal),
   ((if eqb v1 v2 then true else false) = false)->
   v1 <> v2.
-Proof with congruence.
+Proof with try injection; try congruence; intros.
   intros v1 v2 H.
   destruct v1, v2; try discriminate;
   unfold eqb in H;
   unfold eq in H;
-  unfold Rocqlib.zeq in H.
-  - destruct (BinInt.Z.eq_dec (unsigned val) (unsigned val0));
-    try injection...
-  - destruct (BinInt.Z.eq_dec (unsigned base) (unsigned base0));
-    destruct (BinInt.Z.eq_dec (unsigned offset) (unsigned offset0));
-    simpl in *; try injection...        
+  unfold Rocqlib.zeq in H;
+  try injection; try congruence; intros.
+  - destruct val, val0; try congruence;
+    destruct (BinInt.Z.eq_dec (unsigned val) (unsigned val0))...
+  - destruct val, val0; try congruence.
+    destruct (BinInt.Z.eq_dec (unsigned base) (unsigned base0));
+    destruct (BinInt.Z.eq_dec (unsigned idx) (unsigned idx0)); try discriminate;
+    simpl in *.
+    + apply uintw_eq_from_unsigned in e.
+      apply uintw_neq_from_unsigned in n.
+      rewrite e in H1.
+      inversion H1. congruence.
+    + apply uintw_neq_from_unsigned in n.
+      apply uintw_eq_from_unsigned in e.
+      rewrite e in H1.
+      inversion H1. congruence.
+    + apply uintw_neq_from_unsigned in n, n0.
+      inversion H0. congruence.
 Qed.
