SmtExpr.v
@@ -1,11 +1,12 @@
 (* Write out semantics for bitvectors in SMT,
-   show that a single hdr_op evaluation can be converted to the appropriate SMT formula in Z3 *)
+show that a single hdr_op evaluation can be converted to the appropriate SMT formula in Z3 *)
 From MyProject Require Import CrIdentifiers.
 From MyProject Require Import MyInts.
 From MyProject Require Import SmtTypes.
 From MyProject Require Import CrVal.
 From Coq.Strings Require Import String.
 
+(* TODO: Look through K2 code *)
 Inductive SmtBoolExpr : Type :=
     | SmtTrue
     | SmtFalse
@@ -14,7 +15,7 @@ Inductive SmtBoolExpr : Type :=
     | SmtBoolOr (e1 e2 : SmtBoolExpr)
     | SmtBoolEq (e1 e2 : SmtArithExpr)
 with SmtArithExpr : Type :=
-    | SmtConst (value : CrVal)
+    | SmtConst (value : CrInt_T)
     | SmtArithVar (name : string)
     | SmtConditional (cond : SmtBoolExpr) (then_expr else_expr : SmtArithExpr)
     (* Arithmetic operations *)
@@ -27,9 +28,31 @@ with SmtArithExpr : Type :=
     | SmtBitNot (e : SmtArithExpr)
     | SmtBitMul (e1 e2 : SmtArithExpr)
     | SmtBitDiv (e1 e2 : SmtArithExpr)
-    | SmtBitMod (e1 e2 : SmtArithExpr).
+    | SmtBitMod (e1 e2 : SmtArithExpr)
+    | SmtPtrLd (e1 : SmtMemExpr) (e2 : SmtPtrExpr)
+with SmtPtrExpr : Type :=
+    | SmtPtrVal (e1 : CrPtr_T) (* e.g. 0x7fffffff0000 *)
+    | SmtPtrVar (e1 : string) (* e.g. x *)
+    | SmtPtrAdd (e1 : SmtPtrExpr) (e2 : SmtArithExpr)
+with SmtMemExpr : Type :=
+    | SmtMemInit
+    | SmtMemAlloc (e1 : SmtMemExpr) (e2 : SmtPtrExpr)
+    | SmtMemFree (e1 : SmtMemExpr) (e2 : SmtPtrExpr)
+    | SmtPtrSt (e1 : SmtMemExpr) (e2 : SmtPtrExpr) (e3 : SmtArithExpr).
 
 (* Evaluate a SMT Bool expression given a valuation *)
+Definition unwrap_val (v : Check_T CrVal) : CrVal :=
+  match v with
+  | Legal v' => v'
+  | _ => ErrorVal
+  end.
+Transparent unwrap_val.
+Definition unwrap_mem (v : Check_T (Memory CrVal)) : Memory CrVal :=
+  match v with
+  | Legal v' => v'
+  | _ => Invalid
+  end.
+Transparent unwrap_mem.
 Fixpoint eval_smt_bool (e : SmtBoolExpr) (v : SmtValuation) : bool :=
     match e with
     | SmtTrue => true
@@ -37,24 +60,62 @@ Fixpoint eval_smt_bool (e : SmtBoolExpr) (v : SmtValuation) : bool :=
     | SmtBoolNot e' => negb (eval_smt_bool e' v)
     | SmtBoolAnd e1 e2 => andb (eval_smt_bool e1 v) (eval_smt_bool e2 v)
     | SmtBoolOr e1 e2 => orb (eval_smt_bool e1 v) (eval_smt_bool e2 v)
-    | SmtBoolEq e1 e2 => if (CrVal.eqb (eval_smt_arith e1 v) (eval_smt_arith e2 v)) then true else false
+    | SmtBoolEq e1 e2 => if (CrVal.eqb
+      (eval_smt_arith e1 v) (eval_smt_arith e2 v)) then true else false
     end
 with eval_smt_arith (e : SmtArithExpr) (v : SmtValuation) : CrVal :=
-    match e with
-    | SmtConst value => value
-    | SmtArithVar name => v name
-    | SmtConditional cond then_expr else_expr => 
-        if eval_smt_bool cond v 
-        then eval_smt_arith then_expr v 
-        else eval_smt_arith else_expr v
-    | SmtBitAdd e1 e2 => CrVal.add (eval_smt_arith e1 v) (eval_smt_arith e2 v)
-    | SmtBitSub e1 e2 => CrVal.sub (eval_smt_arith e1 v) (eval_smt_arith e2 v)
-    | SmtBitAnd e1 e2 => CrVal.and (eval_smt_arith e1 v) (eval_smt_arith e2 v)
-    | SmtBitOr e1 e2 =>  CrVal.or (eval_smt_arith e1 v) (eval_smt_arith e2 v)
-    | SmtBitXor e1 e2 => CrVal.xor (eval_smt_arith e1 v) (eval_smt_arith e2 v)
-    | SmtBitNot e =>     CrVal.not (eval_smt_arith e v)
-    | SmtBitMul e1 e2 => CrVal.mul (eval_smt_arith e1 v) (eval_smt_arith e2 v)
-    | SmtBitDiv e1 e2 => CrVal.divu (eval_smt_arith e1 v) (eval_smt_arith e2 v)
-    | SmtBitMod e1 e2 => CrVal.modu (eval_smt_arith e1 v) (eval_smt_arith e2 v)
+    unwrap_val match e with
+    | SmtConst value => Legal (IntVal value)
+    | SmtArithVar name => match v name with
+      | IntVal v' => Legal (IntVal v')
+      | _ => Illegal
+      end
+    | SmtConditional cond then_expr else_expr => Legal
+        (if eval_smt_bool cond v 
+        then (eval_smt_arith then_expr v)
+        else (eval_smt_arith else_expr v))
+    | SmtBitAdd e1 e2 => CrVal.add
+        (eval_smt_arith e1 v)
+        (eval_smt_arith e2 v)
+    | SmtBitSub e1 e2 => CrVal.sub
+        (eval_smt_arith e1 v)
+        (eval_smt_arith e2 v)
+    | SmtBitAnd e1 e2 => CrVal.and
+        (eval_smt_arith e1 v)
+        (eval_smt_arith e2 v)
+    | SmtBitOr e1 e2 => CrVal.or
+        (eval_smt_arith e1 v)
+        (eval_smt_arith e2 v)
+    | SmtBitXor e1 e2 => CrVal.xor
+        (eval_smt_arith e1 v)
+        (eval_smt_arith e2 v)
+    | SmtBitNot e => CrVal.not (eval_smt_arith e v)
+    | SmtBitMul e1 e2 => CrVal.mul
+        (eval_smt_arith e1 v)
+        (eval_smt_arith e2 v)
+    | SmtBitDiv e1 e2 => CrVal.divu
+        (eval_smt_arith e1 v)
+        (eval_smt_arith e2 v)
+    | SmtBitMod e1 e2 => CrVal.modu
+        (eval_smt_arith e1 v)
+        (eval_smt_arith e2 v)
+    | SmtPtrLd e1 e2 => CrVal.ld (eval_smt_mem e1 v) (eval_smt_ptr e2 v)
+    end
+with eval_smt_ptr (e : SmtPtrExpr) (v : SmtValuation) : CrVal :=
+    unwrap_val match e with
+    | SmtPtrVal value => Legal (PtrVal value)
+    | SmtPtrVar name => match v name with
+      | PtrVal v' => Legal (PtrVal v')
+      | _ => Illegal
+      end
+    | SmtPtrAdd e1 e2 => CrVal.add (eval_smt_ptr e1 v) (eval_smt_arith e2 v)
+    end
+with eval_smt_mem (e : SmtMemExpr) (v : SmtValuation) : Memory CrVal :=
+    unwrap_mem match e with
+    | SmtMemInit => Legal (@CrVal.tabula_rasa CrVal)
+    | SmtMemAlloc e1 e2 => CrVal.alloc (eval_smt_mem e1 v) (eval_smt_ptr e2 v)
+    | SmtMemFree e1 e2 => CrVal.free (eval_smt_mem e1 v) (eval_smt_ptr e2 v)
+    | SmtPtrSt e1 e2 e3 => CrVal.st (eval_smt_mem e1 v) (eval_smt_ptr e2 v) (eval_smt_arith e3 v)
     end.
+
 (* InitStatus: might be unnecessary and error prone because Z3 may not map 1-to-1 to this. *)
